Updated code for #151

examples/bug-reports/bug151.fst
@@ -1,18 +1,19 @@
 module Bug151
 
-open Array
+open FStar.Array
+open FStar.Seq
 
-type P: int -> nat -> Type
+assume new type p: int -> nat -> Type
 
-type int_1 = x:int{ P x 1 }
-type int_2 = x:int{ P x 2 }
+type int_1 = x:int{ p x 1 }
+type int_2 = x:int{ p x 2 }
 
 type seq_int_1 = seq int_1
 type seq_int_2 = seq int_2
 
 assume val eval:
-    a:seq int -> len:nat{ len <= length a } -> Tot int
+  a:seq int -> len:nat{ len <= length a } -> Tot int
 
 assume val bla2:
-    a:seq_int_1{ length a = 10 } ->
-    b:seq_int_2{ (length b = length a) /\ ( eval a (length a) = eval b (length b)) }
+  a:seq_int_1 int{ length a = 10 } ->
+  b:seq_int_2{ (length b = length a) /\ (eval a (length a) = eval b (length b)) }
